Add π1 and π2 (WIP)

Translation/PackLifts.v
@@ -33,6 +33,8 @@ Fixpoint llift γ δ (t:sterm)  : sterm :=
     sApp (llift γ δ u) (llift γ δ A) (llift γ (S δ) B) (llift γ δ v)
   | sProd na A B => sProd na (llift γ δ A) (llift γ (S δ) B)
   | sSum na A B => sSum na (llift γ δ A) (llift γ (S δ) B)
+  | sPi1 A B p => sPi1 (llift γ δ A) (llift γ (S δ) B) (llift γ δ p)
+  | sPi2 A B p => sPi2 (llift γ δ A) (llift γ (S δ) B) (llift γ δ p)
   | sEq A u v => sEq (llift γ δ A) (llift γ δ u) (llift γ δ v)
   | sRefl A u => sRefl (llift γ δ A) (llift γ δ u)
   | sJ A u P w v p =>
@@ -91,6 +93,8 @@ Fixpoint rlift γ δ t : sterm :=
     sApp (rlift γ δ u) (rlift γ δ A) (rlift γ (S δ) B) (rlift γ δ v)
   | sProd na A B => sProd na (rlift γ δ A) (rlift γ (S δ) B)
   | sSum na A B => sSum na (rlift γ δ A) (rlift γ (S δ) B)
+  | sPi1 A B p => sPi1 (rlift γ δ A) (rlift γ (S δ) B) (rlift γ δ p)
+  | sPi2 A B p => sPi2 (rlift γ δ A) (rlift γ (S δ) B) (rlift γ δ p)
   | sEq A u v => sEq (rlift γ δ A) (rlift γ δ u) (rlift γ δ v)
   | sRefl A u => sRefl (rlift γ δ A) (rlift γ δ u)
   | sJ A u P w v p =>
@@ -1031,6 +1035,11 @@ Proof.
         replace (#|Δ| + 0)%nat with #|Δ| by omega.
         eapply type_App ; emh.
       - cbn. eapply type_Sum ; emh.
+      - cbn. eapply type_Pi1 ; emh.
+      - cbn. replace #|Δ| with (#|Δ| + 0)%nat by omega.
+        rewrite llift_subst.
+        cbn. replace (#|Δ| + 0)%nat with #|Δ| by omega.
+        eapply type_Pi2 ; emh.
       - cbn. eapply type_Eq ; emh.
       - cbn. eapply type_Refl ; emh.
       - cbn. replace #|Δ| with (#|Δ| + 0)%nat by omega.
@@ -1162,6 +1171,11 @@ Proof.
         replace (#|Δ| + 0)%nat with #|Δ| by omega.
         eapply type_App ; emh.
       - cbn. eapply type_Sum ; emh.
+      - cbn. eapply type_Pi1 ; emh.
+      - cbn. replace #|Δ| with (#|Δ| + 0)%nat by omega.
+        rewrite rlift_subst.
+        cbn. replace (#|Δ| + 0)%nat with #|Δ| by omega.
+        eapply type_Pi2 ; emh.
       - cbn. eapply type_Eq ; emh.
       - cbn. eapply type_Refl ; emh.
       - cbn. replace #|Δ| with (#|Δ| + 0)%nat by omega.
